compiler correctness progress: finish Cevaluate_any_env
i.e. that you can add and remove junk to environments in the
intermediate language semantics.

make doPrim2 return an option so it becomes totally specified

experimentation with THEN1 instead of TRY in the proofscript, and
abstracting out some common bits of tactic. the proof still probably
takes longer than it should to replay.

examples/miniML/compiler/compileCorrectnessScript.sml
@@ -169,8 +169,6 @@ val exp_Cexp_ind = CompileTheory.exp_Cexp_ind
 val v_Cv_ind = CompileTheory.v_Cv_ind
 val v_Cv_cases = CompileTheory.v_Cv_cases
 val sort_Cenv_def = CompileTheory.sort_Cenv_def
-val CevalPrim2_def = CompileTheory.CevalPrim2_def
-val doPrim2_def = CompileTheory.doPrim2_def
 val i0_def = CompileTheory.i0_def
 val Cevaluate_ind = CompileTheory.Cevaluate_ind
 val Cevaluate_strongind = CompileTheory.Cevaluate_strongind
@@ -1376,41 +1374,44 @@ rw[FLOOKUP_DEF,force_dom_DRESTRICT_FUNION,FUNION_DEF,DRESTRICT_DEF,FUN_FMAP_DEF]
   rw[INJ_I] >> metis_tac[] ) >>
 qexists_tac `CLit (Bool F)` >> rw[])
 
-(*
-val Cevaluate_any_env = store_thm(
-"Cevaluate_any_env",
-``∀env exp res. Cevaluate env exp res ⇒ ∀env'. Cevaluate ((force_dom env (free_vars exp) (CLit(Bool F))) ⊌ env') exp res``,
-fs[force_dom_DRESTRICT_FUNION] >>
-ho_match_mp_tac Cevaluate_nice_ind >>
-rw[FOLDL_UNION_BIGUNION,FOLDL_UNION_BIGUNION_paired,
-   FAPPLY_FUPDATE_THM,DRESTRICT_DEF,FUNION_DEF,
-   Cevaluate_con,Cevaluate_list_with_Cevaluate,
-   Cevaluate_tageq,Cevaluate_proj,Cevaluate_mat_cons,Cevaluate_let_cons] >>
-TRY (
+val doPrim2_free_vars = store_thm(
+"doPrim2_free_vars",
+``∀b ty op v1 v2 e. (doPrim2 b ty op v1 v2 = SOME e) ⇒ (free_vars e = {})``,
+ntac 3 gen_tac >>
+Cases >> rw[] >>
+Cases_on `l` >> Cases_on `v2` >> fs[] >>
+Cases_on `l` >> fs[] >> pop_assum mp_tac >> rw[] >>
+rw[])
+val _ = export_rewrites["doPrim2_free_vars"]
+
+val CevalPrim2_free_vars = store_thm(
+"CevalPrim2_free_vars",
+``∀p2 v1 v2 e. (CevalPrim2 p2 v1 v2 = SOME e) ⇒ (free_vars e = {})``,
+Cases >> fs[] >> PROVE_TAC[doPrim2_free_vars])
+val _ = export_rewrites["CevalPrim2_free_vars"]
+
+val less2 = prove(``(0:num < 2) ∧ (1:num < 2)``,srw_tac[ARITH_ss][])
+
+val final1 =
+  qmatch_assum_abbrev_tac `∀env'.  Cevaluate (env0 ⊌ env') ee rr` >>
+  qmatch_abbrev_tac `Cevaluate env1 ee rr` >>
+  qsuff_tac `env0 ⊌ env1 = env1` >- PROVE_TAC[] >>
+  rw[GSYM SUBMAP_FUNION_ABSORPTION] >>
+  rw[Abbr`env0`,Abbr`env1`,SUBMAP_DEF,DRESTRICT_DEF,FUNION_DEF,FUN_FMAP_DEF,pairTheory.UNCURRY] >>
+  fsrw_tac[boolSimps.DNF_ss,SATISFY_ss][FUN_FMAP_DEF,pairTheory.UNCURRY] >>
+  metis_tac[]
+val tac1 =
   match_mp_tac (MP_CANON Cevaluate_list_with_mono) >>
   qmatch_assum_abbrev_tac `Cevaluate_list_with P es res` >>
   qexists_tac `P` >> rw[Abbr`P`] >>
-  qmatch_assum_abbrev_tac `∀env'. Cevaluate (env0 ⊌ env') e r` >>
-  qmatch_abbrev_tac `Cevaluate env1 e r` >>
-  qsuff_tac `env0 ⊌ env1 = env1` >- PROVE_TAC[] >>
-  rw[GSYM SUBMAP_FUNION_ABSORPTION] >>
-  rw[Abbr`env0`,Abbr`env1`,SUBMAP_DEF,DRESTRICT_DEF,FUNION_DEF,FUN_FMAP_DEF] >>
-  srw_tac[boolSimps.DNF_ss,SATISFY_ss][FUN_FMAP_DEF] >>
-  metis_tac[] ) >>
-TRY (
+  final1
+val tac2 =
   fs[Once Cpmatch_FEMPTY] >>
   Cases_on `Cpmatch FEMPTY p (env ' n)` >> fs[] >>
   rw[] >>
   (disj1_tac ORELSE rw[Once Cpmatch_FEMPTY]) >>
-  qmatch_assum_abbrev_tac `∀env'.  Cevaluate (env0 ⊌ env') exp res` >>
-  qmatch_abbrev_tac `Cevaluate env1 exp res` >>
-  qsuff_tac `env0 ⊌ env1 = env1` >- PROVE_TAC[] >>
-  rw[GSYM SUBMAP_FUNION_ABSORPTION] >>
-  rw[Abbr`env0`,Abbr`env1`,SUBMAP_DEF,DRESTRICT_DEF,FUNION_DEF,FUN_FMAP_DEF,pairTheory.UNCURRY] >>
-  srw_tac[boolSimps.DNF_ss][FUN_FMAP_DEF,pairTheory.UNCURRY] >>
-  fsrw_tac[boolSimps.DNF_ss,SATISFY_ss][FUN_FMAP_DEF,pairTheory.UNCURRY] >>
-  metis_tac[] ) >>
-TRY (
+  final1
+val tac3 =
   disj1_tac >>
   qexists_tac `v` >>
   qmatch_assum_abbrev_tac `∀env'. Cevaluate (env0 ⊌ env') exp (Rval v)` >>
@@ -1421,18 +1422,8 @@ TRY (
   rw[Abbr`env0`,Abbr`env1`,Abbr`env2`,SUBMAP_DEF,DRESTRICT_DEF,FUNION_DEF,
      DRESTRICT_FUPDATE,FAPPLY_FUPDATE_THM,FUN_FMAP_DEF] >>
   srw_tac[boolSimps.DNF_ss,SATISFY_ss][FUN_FMAP_DEF] >>
-  metis_tac[] ) >>
-TRY (
-  disj2_tac >>
-  qmatch_assum_abbrev_tac `∀env'. Cevaluate (env0 ⊌ env') exp res` >>
-  qmatch_abbrev_tac `Cevaluate env1 exp res` >>
-  qsuff_tac `(env0 ⊌ env1 = env1)` >- PROVE_TAC[] >>
-  rw[GSYM SUBMAP_FUNION_ABSORPTION] >>
-  rw[Abbr`env0`,Abbr`env1`,SUBMAP_DEF,DRESTRICT_DEF,FUNION_DEF,
-     DRESTRICT_FUPDATE,FAPPLY_FUPDATE_THM] >>
-  srw_tac[boolSimps.DNF_ss,SATISFY_ss][FUN_FMAP_DEF] >>
-  metis_tac[] ) >>
-TRY (
+  metis_tac[]
+val tac4 =
   rw[Once Cevaluate_cases] >>
   qmatch_assum_abbrev_tac `∀env'. Cevaluate (env0 ⊌ env') exp res` >>
   qmatch_abbrev_tac `Cevaluate env1 exp res` >>
@@ -1508,13 +1499,93 @@ TRY (
   TRY (conj_tac >- rw[MAP_ZIP,LENGTH_ZIP]) >>
   rw[MAP_ZIP,LENGTH_ZIP,MEM_MAP,pairTheory.EXISTS_PROD] >>
   rw[FUN_FMAP_DEF] >>
-  rw[DRESTRICT_DEF,FUNION_DEF,FUN_FMAP_DEF] ) >>
-TRY (
+  rw[DRESTRICT_DEF,FUNION_DEF,FUN_FMAP_DEF]
+val tac5 =
+  rw[Once Cevaluate_cases] >>
+  ((disj2_tac >> disj1_tac >>
+    qmatch_assum_abbrev_tac `∀env''. Cevaluate (env0 ⊌ env'') exp (Rval (CClosure env' ns exp'))` >>
+    map_every qexists_tac [`env'`,`ns`,`exp'`])
+   ORELSE
+   (disj2_tac >> disj2_tac >> disj2_tac >> disj1_tac >>
+    qmatch_assum_abbrev_tac `∀env''. Cevaluate (env0 ⊌ env'') exp (Rval (CRecClos env' ns' defs n))` >>
+    map_every qexists_tac [`env'`,`ns'`,`defs`,`n`])
+  ) >>
+  rw[Cevaluate_list_with_Cevaluate] >>
+  fs[Cevaluate_list_with_error] >- (
+    qmatch_abbrev_tac `Cevaluate env1 exp v` >>
+    qsuff_tac `env0 ⊌ env1 = env1` >- metis_tac [] >>
+    rw[GSYM SUBMAP_FUNION_ABSORPTION] >>
+    rw[SUBMAP_DEF,Abbr`env0`,Abbr`env1`,DRESTRICT_DEF,FUNION_DEF,FUN_FMAP_DEF] >>
+    srw_tac[boolSimps.DNF_ss,SATISFY_ss][FUN_FMAP_DEF] >>
+    metis_tac[] ) >>
+  qmatch_assum_rename_tac `nn < LENGTH es`[] >>
+  qexists_tac `nn` >>
+  rw[] >- (
+    qmatch_assum_abbrev_tac `∀env'. Cevaluate (env1 ⊌ env') (EL nn es) (Rerr err)` >>
+    qmatch_abbrev_tac `Cevaluate env2 (EL nn es) (Rerr err)` >>
+    qsuff_tac `env1 ⊌ env2 = env2` >- metis_tac[] >>
+    rw[GSYM SUBMAP_FUNION_ABSORPTION] >>
+    rw[SUBMAP_DEF,Abbr`env1`,Abbr`env2`,DRESTRICT_DEF,FUNION_DEF,FUN_FMAP_DEF] >>
+    srw_tac[boolSimps.DNF_ss,SATISFY_ss][FUN_FMAP_DEF] >>
+    srw_tac[boolSimps.DNF_ss,SATISFY_ss][FUN_FMAP_DEF] >>
+    metis_tac[MEM_EL] ) >>
+  first_x_assum (qspec_then `m` mp_tac) >> rw[] >>
+  qexists_tac `v` >>
+  qmatch_assum_abbrev_tac `∀env'. Cevaluate (env1 ⊌ env') (EL m es) (Rval v)` >>
+  qmatch_abbrev_tac `Cevaluate env2 (EL m es) (Rval v)` >>
+  qsuff_tac `env1 ⊌ env2 = env2` >- metis_tac[] >>
+  rw[GSYM SUBMAP_FUNION_ABSORPTION] >>
+  `m < LENGTH es` by srw_tac[ARITH_ss][] >>
+  rw[SUBMAP_DEF,Abbr`env1`,Abbr`env2`,DRESTRICT_DEF,FUNION_DEF,FUN_FMAP_DEF] >>
+  srw_tac[boolSimps.DNF_ss,SATISFY_ss][FUN_FMAP_DEF] >>
+  srw_tac[boolSimps.DNF_ss,SATISFY_ss][FUN_FMAP_DEF] >>
+  metis_tac[MEM_EL]
+val tac6 =
+  rw[Once Cevaluate_cases] >>
+  disj1_tac >>
+  qmatch_assum_abbrev_tac `∀env'. Cevaluate (env0 ⊌ env') exp (Rval (CLit (Bool b)))` >>
+  qexists_tac `b` >>
+  qunabbrev_tac `b` >>
+  conj_tac >- (
+    qmatch_abbrev_tac `Cevaluate env1 ex re` >>
+    qunabbrev_tac `env0` >>
+    qmatch_assum_abbrev_tac `∀env'. Cevaluate (env0 ⊌ env') ex re` >>
+    qsuff_tac `env0 ⊌ env1 = env1` >- metis_tac[] >>
+    rw[GSYM SUBMAP_FUNION_ABSORPTION] >>
+    rw[Abbr`env0`,Abbr`env1`,SUBMAP_DEF,FUNION_DEF,DRESTRICT_DEF,FUN_FMAP_DEF] >>
+    asm_simp_tac(srw_ss()++boolSimps.DNF_ss++SATISFY_ss)[FUN_FMAP_DEF,MEM_EL,pairTheory.UNCURRY] >>
+    metis_tac[]) >>
+  fs[] >>
+  qunabbrev_tac `env0` >>
+  final1
+
+val Cevaluate_any_env = store_thm(
+"Cevaluate_any_env",
+``∀env exp res. Cevaluate env exp res ⇒ ∀env'. Cevaluate ((force_dom env (free_vars exp) (CLit(Bool F))) ⊌ env') exp res``,
+fs[force_dom_DRESTRICT_FUNION] >>
+ho_match_mp_tac Cevaluate_nice_ind >>
+rw[FOLDL_UNION_BIGUNION,FOLDL_UNION_BIGUNION_paired,
+   FAPPLY_FUPDATE_THM,DRESTRICT_DEF,FUNION_DEF,
+   Cevaluate_con,Cevaluate_list_with_Cevaluate,
+   Cevaluate_tageq,Cevaluate_proj,Cevaluate_mat_cons,Cevaluate_let_cons]
+>- tac1
+>- tac1
+>- PROVE_TAC[]
+>- PROVE_TAC[]
+>- tac2
+>- tac2
+>- tac3
+>- tac3
+>- tac3
+>- (disj2_tac >> final1)
+>- tac4
+>- tac4
+>- (
   unabbrev_all_tac >>
   rw[mk_env_canon] >>
   rw[ALOOKUP_APPEND,ALOOKUP_MAP] >>
-  rw[FLOOKUP_DEF,DRESTRICT_DEF,FUNION_DEF,FUN_FMAP_DEF]) >>
-TRY (
+  rw[FLOOKUP_DEF,DRESTRICT_DEF,FUNION_DEF,FUN_FMAP_DEF])
+>- (
   rw[Once Cevaluate_cases] >>
   disj1_tac >>
   qmatch_assum_abbrev_tac `∀env''. Cevaluate (env0 ⊌ env'') exp (Rval (CClosure env' ns exp'))` >>
@@ -1551,46 +1622,221 @@ TRY (
     srw_tac[boolSimps.DNF_ss,SATISFY_ss][FUN_FMAP_DEF,FOLDL2_FUPDATE_LIST] >>
     srw_tac[boolSimps.DNF_ss,SATISFY_ss][FUN_FMAP_DEF] >>
     metis_tac[MEM_EL]
-   ))) >>
-TRY (
+   )))
+>- tac5
+>- (
   rw[Once Cevaluate_cases] >>
-  disj2_tac >> disj1_tac >>
-  qmatch_assum_abbrev_tac `∀env''. Cevaluate (env0 ⊌ env'') exp (Rval (CClosure env' ns exp'))` >>
-  map_every qexists_tac [`env'`,`ns`,`exp'`] >>
-  rw[Cevaluate_list_with_Cevaluate] >>
-  fs[Cevaluate_list_with_error] >- (
-    qmatch_abbrev_tac `Cevaluate env1 exp v` >>
-    qsuff_tac `env0 ⊌ env1 = env1` >- metis_tac [] >>
+  disj2_tac >> disj2_tac >> disj1_tac >>
+  qmatch_assum_abbrev_tac `∀env''. Cevaluate (env0 ⊌ env'') exp (Rval (CRecClos env' ns' defs n))` >>
+  map_every qexists_tac [`env'`,`ns'`,`defs`,`n`] >>
+  qmatch_assum_rename_tac `EL i defs = (ns,exp')`[] >>
+  map_every qexists_tac [`i`,`ns`,`exp'`] >>
+  fs[Cevaluate_list_with_Cevaluate,Cevaluate_list_with_value] >>
+  qexists_tac `vs` >>
+  rw[] >- (
+    qmatch_assum_abbrev_tac `∀env''. Cevaluate (env0 ⊌ env'') exp (Rval v)` >>
+    qmatch_abbrev_tac `Cevaluate env1 exp (Rval v)` >>
+    qsuff_tac `env0 ⊌ env1 = env1` >- metis_tac[] >>
     rw[GSYM SUBMAP_FUNION_ABSORPTION] >>
-    rw[SUBMAP_DEF,Abbr`env0`,Abbr`env1`,DRESTRICT_DEF,FUNION_DEF,FUN_FMAP_DEF] >>
-    srw_tac[boolSimps.DNF_ss,SATISFY_ss][FUN_FMAP_DEF] >>
+    rw[Abbr`env0`,Abbr`env1`,SUBMAP_DEF,DRESTRICT_DEF,FUNION_DEF,FUN_FMAP_DEF] >>
+    srw_tac[SATISFY_ss][FUN_FMAP_DEF] >>
+    metis_tac[] )
+  >- (
+    qmatch_abbrev_tac `Cevaluate env1 (EL m es) (Rval (EL m vs))` >>
+    first_x_assum (qspec_then `m` mp_tac) >> rw[] >>
+    qunabbrev_tac `env0` >>
+    qmatch_assum_abbrev_tac `∀env''. Cevaluate (env0 ⊌ env'') (EL m es) (Rval (EL m vs))` >>
+    qsuff_tac `env0 ⊌ env1 = env1` >- metis_tac[] >>
+    rw[GSYM SUBMAP_FUNION_ABSORPTION] >>
+    rw[Abbr`env0`,Abbr`env1`,SUBMAP_DEF,DRESTRICT_DEF,FUNION_DEF,FUN_FMAP_DEF] >>
+    fsrw_tac[boolSimps.DNF_ss,SATISFY_ss][FUN_FMAP_DEF,MEM_EL] >>
+    metis_tac[MEM_EL] ) >>
+  qmatch_abbrev_tac `Cevaluate env1 exp' res` >>
+  qunabbrev_tac `env0` >>
+  qmatch_assum_abbrev_tac `∀env''. Cevaluate (env0 ⊌ env'') exp' res` >>
+  qsuff_tac `env0 ⊌ env1 = env1` >- metis_tac[] >>
+  rw[GSYM SUBMAP_FUNION_ABSORPTION] >>
+  rw[Abbr`env0`,Abbr`env1`] >>
+  pop_assum kall_tac >>
+  rw[FOLDL2_FUPDATE_LIST,LET_THM,MAP2_MAP,FST_pair,SND_pair,MAP_ZIP,LENGTH_ZIP,FOLDL_FUPDATE_LIST] >>
+  fs[SUBMAP_DEF] >>
+  qx_gen_tac `x` >>
+  fs[DRESTRICT_DEF,FUNION_DEF,FUNION_DEF,FDOM_FUPDATE_LIST,MEM_MAP,pairTheory.EXISTS_PROD,MEM_ZIP,MEM_EL] >>
+  qmatch_abbrev_tac `A ∨ C ⇒ D` >>
+  qsuff_tac `C ⇒ D` >- metis_tac[] >>
+  unabbrev_all_tac >> strip_tac >>
+  conj_asm1_tac >- (
+    `canonical_env_Cv (CRecClos env' ns' defs n)` by metis_tac [Cevaluate_canonical_envs] >>
+    pop_assum mp_tac >>
+    fs[EVERY_MEM,MEM_MAP,pairTheory.EXISTS_PROD,EXTENSION,MEM_EL] >>
     metis_tac[] ) >>
+  rw[] )
+>- tac5
+>- (
+  rw[Once Cevaluate_cases] >>
+  rpt disj2_tac >>
+  qmatch_assum_abbrev_tac `∀env'. Cevaluate (env0 ⊌ env') exp (Rerr err)` >>
+  qmatch_abbrev_tac `Cevaluate env1 exp (Rerr err)` >>
+  qsuff_tac `env0 ⊌ env1 = env1` >- metis_tac[] >>
+  rw[GSYM SUBMAP_FUNION_ABSORPTION] >>
+  rw[Abbr`env0`,Abbr`env1`,SUBMAP_DEF,FUNION_DEF,DRESTRICT_DEF,FUN_FMAP_DEF] >>
+  fsrw_tac[boolSimps.DNF_ss,SATISFY_ss][FUN_FMAP_DEF,MEM_EL] >>
+  metis_tac[])
+>- (
+  rw[Once Cevaluate_cases] >>
+  fs[Cevaluate_list_with_Cevaluate] >>
+  fs[Cevaluate_list_with_value] >>
+  disj1_tac >>
+  qmatch_assum_abbrev_tac `∀env'. Cevaluate (env0 ⊌ env') exp res` >>
+  map_every qexists_tac [`v1`,`v2`,`exp`] >>
+  conj_tac >- (
+    qx_gen_tac `n` >> strip_tac >>
+    first_x_assum (qspec_then `n` mp_tac) >>
+    rw[] >>
+    qmatch_abbrev_tac `Cevaluate env1 ex re` >>
+    qunabbrev_tac `env0` >>
+    qmatch_assum_abbrev_tac `∀env'. Cevaluate (env0 ⊌ env') ex re` >>
+    qsuff_tac `env0 ⊌ env1 = env1` >- metis_tac[] >>
+    rw[GSYM SUBMAP_FUNION_ABSORPTION] >>
+    `(n = 0) ∨ (n = 1)` by DECIDE_TAC >>
+    rw[Abbr`env0`,Abbr`env1`,SUBMAP_DEF,FUNION_DEF,DRESTRICT_DEF,FUN_FMAP_DEF] >>
+    fsrw_tac[boolSimps.DNF_ss,SATISFY_ss][FUN_FMAP_DEF,MEM_EL,MEM] >>
+    full_simp_tac pure_ss [GSYM (CONJUNCT1 EL)] >>
+    metis_tac[less2]) >>
+  fs[] >>
+  qmatch_abbrev_tac `Cevaluate env1 exp res` >>
+  qsuff_tac `env0 ⊌ env1 = env1` >- metis_tac[] >>
+  rw[GSYM SUBMAP_FUNION_ABSORPTION] >>
+  rw[Abbr`env0`,Abbr`env1`,SUBMAP_DEF,FUNION_DEF,DRESTRICT_DEF,FUN_FMAP_DEF] >>
+  imp_res_tac CevalPrim2_free_vars >>
+  fs[] )
+>- (
+  rw[Once Cevaluate_cases] >>
+  rpt disj2_tac >>
+  fs[Cevaluate_list_with_Cevaluate,Cevaluate_list_with_error] >>
   qexists_tac `n` >>
   rw[] >- (
-    qmatch_assum_abbrev_tac `∀env'. Cevaluate (env1 ⊌ env') (EL n es) (Rerr err)` >>
-    qmatch_abbrev_tac `Cevaluate env2 (EL n es) (Rerr err)` >>
-    qsuff_tac `env1 ⊌ env2 = env2` >- metis_tac[] >>
+    qmatch_assum_abbrev_tac `∀env'. Cevaluate (env0 ⊌ env') exp (Rerr err)` >>
+    qmatch_abbrev_tac `Cevaluate env1 exp (Rerr err)` >>
+    qsuff_tac `env0 ⊌ env1 = env1` >- metis_tac[] >>
     rw[GSYM SUBMAP_FUNION_ABSORPTION] >>
-    rw[SUBMAP_DEF,Abbr`env1`,Abbr`env2`,DRESTRICT_DEF,FUNION_DEF,FUN_FMAP_DEF] >>
-    srw_tac[boolSimps.DNF_ss,SATISFY_ss][FUN_FMAP_DEF] >>
-    srw_tac[boolSimps.DNF_ss,SATISFY_ss][FUN_FMAP_DEF] >>
-    metis_tac[MEM_EL] ) >>
+    `(n = 0) ∨ (n = 1)` by DECIDE_TAC >>
+    rw[Abbr`env0`,Abbr`env1`,Abbr`exp`,SUBMAP_DEF,FUNION_DEF,DRESTRICT_DEF,FUN_FMAP_DEF] >>
+    fsrw_tac[boolSimps.DNF_ss,SATISFY_ss][FUN_FMAP_DEF,MEM_EL] >>
+    metis_tac[]) >>
   first_x_assum (qspec_then `m` mp_tac) >> rw[] >>
   qexists_tac `v` >>
-  qmatch_assum_abbrev_tac `∀env'. Cevaluate (env1 ⊌ env') (EL m es) (Rval v)` >>
-  qmatch_abbrev_tac `Cevaluate env2 (EL m es) (Rval v)` >>
-  qsuff_tac `env1 ⊌ env2 = env2` >- metis_tac[] >>
+  qmatch_assum_abbrev_tac `∀env'. Cevaluate (env0 ⊌ env') exp (Rval v)` >>
+  qmatch_abbrev_tac `Cevaluate env1 exp (Rval v)` >>
+  qsuff_tac `env0 ⊌ env1 = env1` >- metis_tac[] >>
   rw[GSYM SUBMAP_FUNION_ABSORPTION] >>
+  `(m = 0) ∨ (m = 1)` by DECIDE_TAC >>
+  rw[Abbr`env0`,Abbr`env1`,Abbr`exp`,SUBMAP_DEF,FUNION_DEF,DRESTRICT_DEF,FUN_FMAP_DEF] >>
+  fsrw_tac[boolSimps.DNF_ss,SATISFY_ss][FUN_FMAP_DEF,MEM_EL] >>
+  metis_tac[])
+>- (
+  rw[Once Cevaluate_cases] >>
+  fs[Cevaluate_list_with_Cevaluate] >>
+  fs[Cevaluate_list_with_value] >>
+  disj1_tac >>
+  qmatch_assum_abbrev_tac `∀env'. Cevaluate (env0 ⊌ env') exp res` >>
+  map_every qexists_tac [`v1`,`v2`,`exp`] >>
+  conj_tac >- (
+    qx_gen_tac `n` >> strip_tac >>
+    first_x_assum (qspec_then `n` mp_tac) >>
+    rw[] >>
+    qmatch_abbrev_tac `Cevaluate env1 ex re` >>
+    qunabbrev_tac `env0` >>
+    qmatch_assum_abbrev_tac `∀env'. Cevaluate (env0 ⊌ env') ex re` >>
+    qsuff_tac `env0 ⊌ env1 = env1` >- metis_tac[] >>
+    rw[GSYM SUBMAP_FUNION_ABSORPTION] >>
+    `(n = 0) ∨ (n = 1)` by DECIDE_TAC >>
+    rw[Abbr`env0`,Abbr`env1`,SUBMAP_DEF,FUNION_DEF,DRESTRICT_DEF,FUN_FMAP_DEF] >>
+    `x ∈ BIGUNION (IMAGE free_vars (set es))` by (
+      rw[] >> qexists_tac `free_vars ex` >> rw[] >>
+      qexists_tac `ex` >>
+      rw[Abbr`ex`] >>
+      Cases_on `es` >> fs[] >>
+      Cases_on `t` >> fs[]) >>
+    `FINITE (BIGUNION (IMAGE free_vars (set es)))` by (
+      rw[] >> rw[] ) >>
+    asm_simp_tac(srw_ss()++boolSimps.DNF_ss++SATISFY_ss)[FUN_FMAP_DEF,MEM_EL,pairTheory.UNCURRY] >>
+    metis_tac[less2]) >>
+  fs[] >>
+  qmatch_abbrev_tac `Cevaluate env1 exp res` >>
+  qsuff_tac `env0 ⊌ env1 = env1` >- metis_tac[] >>
+  rw[GSYM SUBMAP_FUNION_ABSORPTION] >>
+  rw[Abbr`env0`,Abbr`env1`,SUBMAP_DEF,FUNION_DEF,DRESTRICT_DEF,FUN_FMAP_DEF] >>
+  imp_res_tac doPrim2_free_vars >>
+  fs[] )
+>- (
+  rw[Once Cevaluate_cases] >>
+  rpt disj2_tac >>
+  fs[Cevaluate_list_with_Cevaluate,Cevaluate_list_with_error] >>
+  qexists_tac `n` >>
+  rw[] >- (
+    qmatch_assum_abbrev_tac `∀env'. Cevaluate (env0 ⊌ env') exp (Rerr err)` >>
+    qmatch_abbrev_tac `Cevaluate env1 exp (Rerr err)` >>
+    qsuff_tac `env0 ⊌ env1 = env1` >- metis_tac[] >>
+    rw[GSYM SUBMAP_FUNION_ABSORPTION] >>
+    rw[Abbr`env0`,Abbr`env1`,Abbr`exp`,SUBMAP_DEF,FUNION_DEF,DRESTRICT_DEF,FUN_FMAP_DEF] >>
+    fsrw_tac[boolSimps.DNF_ss,SATISFY_ss][FUN_FMAP_DEF,MEM_EL] >>
+    metis_tac[]) >>
+  first_x_assum (qspec_then `m` mp_tac) >> rw[] >>
   `m < LENGTH es` by srw_tac[ARITH_ss][] >>
-  rw[SUBMAP_DEF,Abbr`env1`,Abbr`env2`,DRESTRICT_DEF,FUNION_DEF,FUN_FMAP_DEF] >>
-  srw_tac[boolSimps.DNF_ss,SATISFY_ss][FUN_FMAP_DEF] >>
-  srw_tac[boolSimps.DNF_ss,SATISFY_ss][FUN_FMAP_DEF] >>
-  metis_tac[MEM_EL] ) >>
+  qexists_tac `v` >>
+  qmatch_assum_abbrev_tac `∀env'. Cevaluate (env0 ⊌ env') exp (Rval v)` >>
+  qmatch_abbrev_tac `Cevaluate env1 exp (Rval v)` >>
+  qsuff_tac `env0 ⊌ env1 = env1` >- metis_tac[] >>
+  rw[GSYM SUBMAP_FUNION_ABSORPTION] >>
+  rw[Abbr`env0`,Abbr`env1`,Abbr`exp`,SUBMAP_DEF,FUNION_DEF,DRESTRICT_DEF,FUN_FMAP_DEF] >>
+  fsrw_tac[boolSimps.DNF_ss,SATISFY_ss][FUN_FMAP_DEF,MEM_EL] >>
+  metis_tac[])
+>- tac6
+>- tac6
+>- (
+  rw[Once Cevaluate_cases] >>
+  disj2_tac >>
+  final1 )
+>- (
+  rw[Once Cevaluate_cases] >>
+  disj1_tac >>
+  final1 )
+>- (
+  rw[Once Cevaluate_cases] >>
+  disj2_tac >>
+  disj1_tac >>
+  conj_tac >- (
+    pop_assum kall_tac >>
+    final1 ) >>
+  final1 )
+>- (
+  rw[Once Cevaluate_cases] >>
+  disj2_tac >>
+  final1 )
+>- (
+  rw[Once Cevaluate_cases] >>
+  disj1_tac >>
+  final1 )
+>- (
+  rw[Once Cevaluate_cases] >>
+  disj2_tac >> disj1_tac >>
+  conj_tac >- (
+    pop_assum kall_tac >>
+    final1 ) >>
+  final1 )
+>- (
+  rw[Once Cevaluate_cases] >>
+  disj2_tac >>
+  final1 )
+>- rw[Cevaluate_list_with_cons]
+>- rw[Cevaluate_list_with_cons]
+>- (
+  rw[Cevaluate_list_with_cons] >>
+  disj1_tac >>
+  qexists_tac `v` >>
+  rw[] ))
 
->> PROVE_TAC[]
-*)
-
-(*
 val Cevaluate_free_vars_env = save_thm(
 "Cevaluate_free_vars_env",
 Cevaluate_any_env
@@ -1600,7 +1846,6 @@ Cevaluate_any_env
 |> SIMP_RULE (srw_ss()) [FUNION_FEMPTY_2]
 |> DISCH_ALL
 |> Q.GEN `res` |> Q.GEN `exp` |> Q.GEN `env`)
-*)
 
 (* Prove compiler phases preserve semantics *)
 
