examples/miniML/compiler/compileTerminationScript.sml
@@ -136,6 +136,12 @@ val _ = export_rewrites["Cmatch_map_def"];
 val _ = save_thm ("Cmatch_bind_def", Cmatch_bind_def);
 val _ = export_rewrites["Cmatch_bind_def"];
 
+val _ = save_thm ("doPrim2_def", doPrim2_def);
+val _ = export_rewrites["doPrim2_def"];
+
+val _ = save_thm ("CevalPrim2_def", CevalPrim2_def);
+val _ = export_rewrites["CevalPrim2_def"];
+
 val (Cpmatch_def,Cpmatch_ind) = register "Cpmatch" (
   tprove_no_defn ((Cpmatch_def,Cpmatch_ind),
   WF_REL_TAC `inv_image $<
